limit refinement

theories/Compositional_Structures/Basic_Modules/Borda_Module_Ref.thy
@@ -5,10 +5,7 @@ begin
 
 fun borda_score_mon :: "'a Evaluation_Function_Ref" where
   "borda_score_mon x A p =
-    FOREACH A (\<lambda> y sc. do {
-      pcx <- prefer_count_monadic_imp p x y; 
-      RETURN (sc + pcx)})
-    (0::nat)"
+    sum_impl (prefer_count_monadic_imp p x) A"
 
 definition borda_monadic :: "'a Electoral_Module_Ref" where
   "borda_monadic A pl \<equiv> do {
@@ -24,36 +21,15 @@ lemma borda_score_refine_alt:
     and profrel: "(pl, pr) \<in> profile_rel"
   shows "borda_score_mon x A pl \<le> SPEC (\<lambda> sc. sc = (borda_score x A pr))"
   unfolding borda_score_mon.simps borda_score.simps
-  apply (refine_vcg FOREACH_rule[where I = 
-          "(\<lambda>it sc. sc = (\<Sum> y \<in> (A - it). (prefer_count pr x y)))"])
-     apply (auto simp add: fina simp del:  prefer_count.simps)
-proof (-)
-  fix xa :: 'a
-  fix it :: "'a set"
-  assume xit: "xa \<in> it"
-  assume itA: "it \<subseteq> A"
-  from profrel have "(pl, pr) \<in> profile_rel" using profile_type_ref
-    by fastforce
-  from this have pcref: "prefer_count_monadic_imp pl x xa 
-        \<le> SPEC (\<lambda> pcxa. pcxa = prefer_count pr x xa)" 
-    using prefer_count_monadic_imp_correct by fastforce
-  from fina itA xit have "sum (prefer_count pr x) (A - it) + (prefer_count pr x xa)
-    = sum (prefer_count pr x) (A - (it - {xa}))"
-  by (metis Diff_iff ab_semigroup_add_class.add.commute finite_Diff it_step_insert_iff sum.insert)
-  from pcref this show "prefer_count_monadic_imp pl x xa
-       \<le> SPEC (\<lambda>pcx. sum (prefer_count pr x) (A - it) + pcx =
-                      sum (prefer_count pr x) (A - (it - {xa})))"
-    by (metis (mono_tags, lifting) SPEC_cons_rule)
-qed
-
+  by (refine_vcg fina sum_impl_correct prefer_count_monadic_imp_correct  profrel)
+ 
 
 lemma borda_score_correct:
   shows "(borda_score_mon, borda_score)
     \<in> evalf_rel"
-  apply (auto simp add: evalf_rel_def simp del: borda_score_mon.simps
-      borda_score.simps)
-  apply (refine_vcg)
-proof (unfold borda_score_mon.simps, rename_tac x A' A pl pr)
+  unfolding evalf_rel_def
+proof (clarify, refine_rcg, unfold borda_score_mon.simps borda_score.simps, 
+        rename_tac x A' A pl pr)
   fix A' A :: "'a set"
   fix x :: 'a
   fix pl :: "'a Profile_List"
@@ -62,92 +38,12 @@ proof (unfold borda_score_mon.simps, rename_tac x A' A pl pr)
   assume prel: "(pl, pr) \<in> profile_rel"
   from arel have aeq: "A' = A" by (auto simp add: alt_set_rel_def in_br_conv)
   from arel have fina: "finite A'" by (auto simp add: alt_set_rel_def in_br_conv)
-  from this 
-  show "FOREACH A' (\<lambda>y sc. prefer_count_monadic_imp pl x y \<bind> (\<lambda>pcx. RETURN (sc + pcx))) 0
-       \<le> SPEC (\<lambda>c. (c, borda_score x A pr) \<in> nat_rel)"
-  proof (refine_vcg FOREACH_rule[where I = 
-        "(\<lambda>it sc. sc = (\<Sum> y \<in> (A - it). (prefer_count pr x y)))"],
-      clarsimp_all simp add: fina aeq simp del:  prefer_count.simps)
-    fix xa :: 'a
-    fix it :: "'a set"
-    assume xit: "xa \<in> it"
-    assume itA: "it \<subseteq> A"
-    from prel have pcref: "prefer_count_monadic_imp pl x xa 
-        \<le> SPEC (\<lambda> pcxa. pcxa = prefer_count pr x xa)" 
-    using prefer_count_monadic_imp_correct by fastforce
-    from fina itA xit aeq have "sum (prefer_count pr x) (A - it) + (prefer_count pr x xa)
-      = sum (prefer_count pr x) (A - (it - {xa}))"
-      by (metis Diff_iff ab_semigroup_add_class.add.commute finite_Diff it_step_insert_iff sum.insert)
-    from pcref this show "prefer_count_monadic_imp pl x xa
-       \<le> SPEC (\<lambda>pcx. sum (prefer_count pr x) (A - it) + pcx =
-                      sum (prefer_count pr x) (A - (it - {xa})))"
-    by (metis (mono_tags, lifting) SPEC_cons_rule)
-  qed
+  show "sum_impl (prefer_count_monadic_imp pl x) A' \<le> SPEC (\<lambda>sc. sc = sum (prefer_count pr x) A)"
+    by (refine_vcg fina prel prefer_count_monadic_imp_correct sum_impl_correct, simp add: aeq)
 qed
 
 
 theorem borda_ref_correct:          
-  shows "(borda_monadic, borda) \<in> em_rel"
-  unfolding em_rel_def borda_monadic_def borda.simps
-proof (clarify, rename_tac A' A pl pr)
-  fix A' A:: "'a set"
-  fix pl :: "'a Profile_List"
-  fix pr :: "'a Profile"
-  assume arel: "(A', A) \<in> \<langle>Id\<rangle>alt_set_rel"
-  assume prel: " (pl, pr) \<in> profile_rel"
-  from arel have aeq: "A' = A" by (auto simp add: alt_set_rel_def in_br_conv)
-  from arel have fina: "finite A'" by (auto simp add: alt_set_rel_def in_br_conv)
-  note compute_scores_correct[THEN fun_relD, THEN fun_relD, THEN fun_relD, THEN nres_relD, 
-          THEN refine_IdD, where x4 = borda_score_mon and x'4 = borda_score]
-  from arel prel this borda_score_correct have 
-    precompborda: "pre_compute_scores borda_score_mon A' pl
-  \<le> SPEC (\<lambda>map. map = pre_computed_map borda_score A pr)" by fastforce
-  note maxelim = max_eliminator_ref_correct[where efn = borda_score, THEN fun_relD]
-  from arel aeq prel precompborda this show "(pre_compute_scores borda_score_mon A' pl \<bind>
-        (\<lambda>scores. max_eliminator_ref scores A' pl),
-        SPEC (\<lambda>res. res = max_eliminator borda_score A pr))
-       \<in> \<langle>\<langle>Id\<rangle>set_rel \<times>\<^sub>r \<langle>Id\<rangle>set_rel \<times>\<^sub>r \<langle>Id\<rangle>set_rel\<rangle>nres_rel"
-    using specify_left[where M = 
-        "\<Down> (\<langle>Id\<rangle>set_rel \<times>\<^sub>r \<langle>Id\<rangle>set_rel \<times>\<^sub>r \<langle>Id\<rangle>set_rel) 
-  (SPEC (\<lambda>res. res = max_eliminator borda_score A pr))"
-       and m = "pre_compute_scores borda_score_mon A' pl"
-       and \<Phi> = "(\<lambda>map. map = pre_computed_map borda_score A pr)"
-       and f = "(\<lambda>scores. max_eliminator_ref scores A' pl)"]
-  nres_relI nres_relD by blast
-qed 
-    
-
-abbreviation "profile_impl_assn \<equiv> (list_assn (array_assn nat_assn))"
-
-abbreviation "alts_set_impl_assn \<equiv> (hs.assn nat_assn)"
-
-abbreviation "result_assn \<equiv> alts_set_impl_assn \<times>\<^sub>a alts_set_impl_assn \<times>\<^sub>a alts_set_impl_assn"
-
-find_theorems id_assn
-
-sepref_definition borda_elim_sepref is
-  "uncurry borda_monadic":: 
-    "(hs.assn nat_assn)\<^sup>k *\<^sub>a (list_assn (array_assn nat_assn))\<^sup>k 
-   \<rightarrow>\<^sub>a (result_assn)"
-  unfolding borda_monadic_def  max_eliminator_ref.simps borda_score_mon.simps
-    less_eliminator_ref.simps  elimination_module_ref_def[abs_def] eliminate_def[abs_def]
-    pre_compute_scores_def[abs_def] scoremax_def[abs_def] 
-    prefer_count_monadic_imp_def[abs_def] is_less_preferred_than_mon_def[abs_def]
-    rank_mon_def[abs_def] index_mon_def[abs_def]
-    short_circuit_conv
-  apply (rewrite in "FOREACH _ _ \<hole>" hm.fold_custom_empty)
-  apply (rewrite in "FOREACH _ _ \<hole>" hs.fold_custom_empty)
-  apply (rewrite in "FOREACH _ _ \<hole>" hs.fold_custom_empty)
-  apply (rewrite in "_ \<bind> (\<lambda>(rej, def). if def = {} then RETURN (\<hole>, _, rej) else RETURN ({}, rej, def))" hs.fold_custom_empty)
-  apply (rewrite in "_ \<bind> (\<lambda>(rej, def). if def = {} then RETURN (_, \<hole>, rej) else RETURN ({}, rej, def))" hs.fold_custom_empty)
-  apply (rewrite in "_ \<bind> (\<lambda>(rej, def). if def = {} then RETURN (_, _, rej) else RETURN (\<hole>, rej, def))" hs.fold_custom_empty)
-
-  apply sepref_dbg_keep
-
-  done
-
-
-theorem borda_sep_aux:          
   shows "(borda_monadic,(\<lambda> A p. SPEC (\<lambda> em. em = borda A p))) \<in> elec_mod_relb"
   unfolding borda_monadic_def borda.simps
 proof (clarify, rename_tac A' A pl pr)
@@ -176,8 +72,47 @@ proof (clarify, rename_tac A' A pl pr)
        and f = "(\<lambda>scores. max_eliminator_ref scores A' pl)"]
   nres_relI nres_relD by blast
 qed 
-  
 
-lemmas borda_sepref_correct =  borda_elim_sepref.refine[FCOMP borda_sep_aux]
+abbreviation "profile_impl_assn \<equiv> (list_assn (arl_assn nat_assn))"
+
+abbreviation "alts_set_impl_assn \<equiv> (hs.assn nat_assn)"
+
+abbreviation "result_impl_assn \<equiv> alts_set_impl_assn \<times>\<^sub>a alts_set_impl_assn \<times>\<^sub>a alts_set_impl_assn"
+
+definition "alts_assn \<equiv> hr_comp (hs.assn nat_assn) (\<langle>nat_rel\<rangle>alt_set_rel)"
+
+definition "profile_assn \<equiv> (list_assn (hr_comp (list_assn nat_assn) ballot_rel))"
+
+abbreviation "result_assn \<equiv> hr_comp (hs.assn nat_assn) (\<langle>nat_rel\<rangle>set_rel) \<times>\<^sub>a
+                               hr_comp (hs.assn nat_assn) (\<langle>nat_rel\<rangle>set_rel) \<times>\<^sub>a
+                               hr_comp (hs.assn nat_assn) (\<langle>nat_rel\<rangle>set_rel)"
+
+
+
+sepref_definition borda_elim_sepref is
+  "uncurry borda_monadic":: 
+    "alts_set_impl_assn\<^sup>k *\<^sub>a (profile_impl_assn)\<^sup>k 
+   \<rightarrow>\<^sub>a (result_impl_assn)"
+  unfolding borda_monadic_def  max_eliminator_ref.simps borda_score_mon.simps sum_impl_def
+    less_eliminator_ref.simps  elimination_module_ref_def[abs_def] eliminate_def[abs_def]
+    pre_compute_scores_def[abs_def] scoremax_def[abs_def] 
+    prefer_count_monadic_imp_def[abs_def] is_less_preferred_than_mon_def[abs_def]
+    rank_mon_def[abs_def] index_mon_def[abs_def]
+    short_circuit_conv
+  apply (rewrite in "FOREACH _ _ \<hole>" hm.fold_custom_empty)
+  apply (rewrite in "FOREACH _ _ \<hole>" hs.fold_custom_empty)
+  apply (rewrite in "FOREACH _ _ \<hole>" hs.fold_custom_empty)
+  apply (rewrite in "_ \<bind> (\<lambda>(rej, def). if def = {} then RETURN (\<hole>, _, rej) else RETURN ({}, rej, def))" hs.fold_custom_empty)
+  apply (rewrite in "_ \<bind> (\<lambda>(rej, def). if def = {} then RETURN (_, \<hole>, rej) else RETURN ({}, rej, def))" hs.fold_custom_empty)
+  apply (rewrite in "_ \<bind> (\<lambda>(rej, def). if def = {} then RETURN (_, _, rej) else RETURN (\<hole>, rej, def))" hs.fold_custom_empty)
+
+  apply sepref_dbg_keep
+
+  done
+       
+
+
+lemmas borda_impl_correct = borda_elim_sepref.refine[FCOMP borda_ref_correct]
+  
 
 end
